equational_theories/MemoFinOp.lean
@@ -9,41 +9,39 @@ namespace MemeFinOp
 
 open Lean Meta Elab Term
 
-def opOfTable {n : Nat} (s t : Nat) (a : Fin n) (b : Fin n) : Fin n :=
-  ⟨(t >>> (s * (a.val * n + b.val))) % n, Nat.mod_lt _ (Fin.pos a)⟩
+def opOfTable {n : Nat} (t : Nat) (a : Fin n) (b : Fin n) : Fin n :=
+  let i := a.val * n + b.val
+  let r := (t / n^i) % n
+  ⟨r, Nat.mod_lt _ (Fin.pos a)⟩
 
 /-- `enum n` is the array of all elements of `Fin n` in order -/
-private def Fin.enum (n) : Array (Fin n) := Array.ofFn Fin.rev
+private def Fin.enum (n) : Array (Fin n) := Array.ofFn id
 
-def buildMemo {n : Nat} (f : Fin n → Fin n → Fin n) : Nat × Nat := Id.run do
-  let s := 1 + Nat.log2 (n-1)
+def buildMemo {n : Nat} (f : Fin n → Fin n → Fin n) : Nat := Id.run do
   let mut t := 0
-  let mut last := 0
   for a in Fin.enum n do
     for b in Fin.enum n do
-      let ne := f a b
-      t := (t <<< s) + (ne + n - (last <<< s) % n) % n
-      last := ne
-
-  (t, s)
+      let i := a.val * n + b.val
+      t := t + f a b * n^i
+  t
 
 -- Quick sanity check:
 example :
     let f := fun (a b : Fin 4) => a * a * b + 2
-    opOfTable (buildMemo f).2 (buildMemo f).1 = f := by
+    opOfTable (buildMemo f) = f := by
   funext a b; revert a b; native_decide
 
-private unsafe def evalNatProdImpl (e : Expr) : MetaM (Nat × Nat) := do
+private unsafe def evalNatImpl (e : Expr) : MetaM Nat := do
   let t ← inferType e
-  unless t.isAppOfArity ``Prod 2 && (t.getArg! 1).isConstOf ``Nat && (t.getArg! 2).isConstOf ``Nat do
-    throwError "evalNat: expected expression of type `Nat × Nat`, but got {t}"
+  unless t.isConstOf ``Nat do
+    throwError "evalNat: expected expression of type `Nat`, but got {t}"
   let e ← instantiateMVars e
   if e.hasExprMVar then
     throwError "evalNat: cannot evaluate expression{indentExpr e}\nit contains metavariables"
-  evalExpr (Nat × Nat) (← mkAppM ``Prod #[mkConst ``Nat, mkConst ``Nat]) e
+  evalExpr Nat (mkConst ``Nat) e
 
-@[implemented_by evalNatProdImpl]
-private opaque evalNatProd (value : Expr) : MetaM (Nat × Nat)
+@[implemented_by evalNatImpl]
+private opaque evalNat (value : Expr) : MetaM Nat
 
 /-
 The syntax `memoFinOp f` takes a function `f : Fin n → Fin n → Fin n` and implements it in a
@@ -74,8 +72,8 @@ elab "memoFinOp" fn:term:arg :term <= expectedType? => do
     throwError "expected type {expectedType}, got {type}"
 
   -- Tabulation
-  let table ← evalNatProd (mkApp2 (mkConst ``buildMemo) nE fn)
-  return mkApp3 (mkConst ``opOfTable) nE (.lit (.natVal table.snd)) (.lit (.natVal table.fst))
+  let table ← evalNat (mkApp2 (mkConst ``buildMemo) nE fn)
+  return mkApp2 (mkConst ``opOfTable) nE (.lit (.natVal table))
 
 example :
     let f := fun (a b : Fin 4) => a * a * b + (2 : Fin 4)
